@prefix rdf: <http://www.w3.org/1999/02/22-rdf-syntax-ns#> .
@prefix rdfs: <http://www.w3.org/2000/01/rdf-schema#> .
@prefix lite: <http://bibfra.me/vocab/lite/> .
@prefix rel: <http://bibfra.me/vocab/relation/> .
@prefix dc: <http://purl.org/dc/terms/> .
@prefix schema: <http://schema.org/> .
@prefix owl: <http://www.w3.org/2002/07/owl#> .
@prefix bf: <http://id.loc.gov/ontologies/bibframe/> .
@prefix skos: <http://www.w3.org/2004/02/skos/core#> .
@prefix oa: <http://www.w3.org/ns/oa#> .
@prefix foaf: <http://xmlns.com/foaf/0.1/> .

# BIBFRAME Linked Data Extension aka BUILDE Relation üìñüîç

# This RDF vocabulary encompasses a wide range of classes and properties suitable for describing various
# types of bibliographic resources, scholarly works, and related entities. BUILDE includes a basic set of 
# core classes and properties known as the 'lite' layer described here, as well as several extensions:

#	archive: things found in archives
#	rare books: things found in rare book libraries
#	scholar: things found in scholarly research and publishing
#	library: things found in libraries

# This vocabulary is ideal for librarians, information scientists, data curators, and developers working
# in academic and research settings. It can be employed in creating digital libraries, scholarly databases,
# cataloging systems, and other applications requiring structured bibliographic information.

# Key Features:
# - Compatibility with existing ontologies including Schema.org, SKOS, FOAF, and Dublin Core for enhanced interoperability.
# - Extension of BIBFRAME from the Library of Congress
# - Comprehensive coverage of bibliographic and scholarly domains.
# - Clear, self-explanatory labels and definitions for each class and property.
# - Hierarchical organization of classes using rdfs:subClassOf for structured representation.

# We encourage users to provide feedback and suggestions to continually improve and update this vocabulary.
# For versioning, updates, and more detailed documentation, please visit [https://bibfra.me/?].

# ------------------------------
# Created by: EBSCO Information Systems
# Version: 1.0
# Created: July 30, 2024
# Updated: July 30, 2024
# ------------------------------

## Relationships between Works

rel:absorbed a rdf:Property ;
    rdfs:label "absorbed"@en ;
    rdfs:comment "Work that has been incorporated into another Work."@en ;
    rdfs:domain lite:Resource ;
    rdfs:range lite:Resource .

rel:absorbedBy a rdf:Property ;
    rdfs:label "absorbed by"@en ;
    rdfs:comment "Resource was absorbed by another resource."@en ;
    rdfs:domain lite:Resource ;
    rdfs:range lite:Resource .

rel:absorbedInPart a rdf:Property ;
    rdfs:label "absorbed in part"@en ;
    rdfs:comment "Work that has been partially incorporated into another work."@en ;
    rdfs:domain lite:Resource ;
    rdfs:range lite:Resource .

rel:absorbedInPartBy a rdf:Property ;
    rdfs:label "absorbed in part by"@en ;
    rdfs:comment "Resource was partially absorbed by another resource."@en ;
    rdfs:domain lite:Resource ;
    rdfs:range lite:Resource .

rel:changedBackTo a rdf:Property ;
    rdfs:label "changed back to"@en ;
    rdfs:comment "Work that has been changed back into another work."@en ;
    rdfs:domain lite:Resource ;
    rdfs:range lite:Resource .

rel:continueBy a rdf:Property ;
    rdfs:label "continue by"@en ;
    rdfs:comment "Work whose content continues an earlier work under a new title."@en ;
    rdfs:domain lite:Resource ;
    rdfs:range lite:Resource .

rel:continues a rdf:Property ;
    rdfs:label "continues"@en ;
    rdfs:comment "Work that is continued by the content of a later work under a new title."@en ;
    rdfs:domain lite:Resource ;
    rdfs:range lite:Resource .

rel:continuesInPart a rdf:Property ;
    rdfs:label "continues in part"@en ;
    rdfs:comment "Work that split into two or more separate works with new titles."@en ;
    rdfs:domain lite:Resource ;
    rdfs:range lite:Resource .

rel:continuedInPartBy a rdf:Property ;
    rdfs:label "continued in part by"@en ;
    rdfs:comment "Content of a previous resource is partially continued in a new resource."@en ;
    rdfs:domain lite:Resource ;
    rdfs:range lite:Resource .

rel:hasBasis a rdf:Property ;
    rdfs:label "has basis"@en ;
    rdfs:comment "Trarget resource is the basis of the source resource."@en ;
    rdfs:range lite:Resource ;
    rdfs:domain lite:Resource .

rel:hasDerivative a rdf:Property ;
    rdfs:label "has derivative"@en ;
    rdfs:comment "Target resource is a modification of the source resource."@en ;
    rdfs:range lite:Resource ;
    rdfs:domain lite:Resource .

rel:hasEdition a rdf:Property ;
    rdfs:label "has edition"@en ;
    rdfs:comment "Target resource is a particular version of a source resource that has been revised or created."@en ;
    rdfs:range lite:Resource ;
    rdfs:domain lite:Resource .

rel:hasExpression a rdf:Property ;
    rdfs:label "has expression"@en ;
    rdfs:comment "Resource has a related expression. For use to connect Works under FRBR/RDA rules."@en ;
    rdfs:range lite:Resource ;
    rdfs:domain lite:Resource .

rel:hasEquivalent a rdf:Property ;
    rdfs:label "has equivalent"@en ;
    rdfs:comment "Embodies the same as the resource being described."@en ;
    rdfs:range lite:Resource ;
    rdfs:domain lite:Resource .

rel:hasPart a rdf:Property ;
    rdfs:label "has part"@en ;
    rdfs:comment "Resource that is included either physically or logically contained in the described resource."@en ;
    rdfs:range lite:Resource ;
    rdfs:domain lite:Resource .

rel:isAdaptationOf a rdf:Property ;
    rdfs:label "is adaptation of"@en ;
    rdfs:comment "Source resource is an adaptation of the target resource."@en ;
    rdfs:range lite:Resource ;
    rdfs:domain lite:Resource .

rel:isBasedOn a rdf:Property ;
    rdfs:label "is based on"@en ;
    rdfs:comment "Source resource is based on the target resource."@en ;
    rdfs:range lite:Resource ;
    rdfs:domain lite:Resource .

rel:isDerivativeOf a rdf:Property ;
    rdfs:label "is derivative of"@en ;
    rdfs:comment "Source resource is a modification of the target resource."@en ;
    rdfs:range lite:Resource ;
    rdfs:domain lite:Resource .

rel:isEditionOf a rdf:Property ;
    rdfs:label "is edition of"@en ;
    rdfs:comment "Source resource is a particular version of a target resource that has been revised or created."@en ;
    rdfs:range lite:Resource ;
    rdfs:domain lite:Resource .

rel:isPartOf a rdf:Property ;
    rdfs:label "is part of"@en ;
    rdfs:comment "Relationship that connects things that are part of other things."@en ;
    rdfs:range lite:Resource ;
    rdfs:domain lite:Resource .

rel:isTranslationOf a rdf:Property ;
    rdfs:label "is translation of"@en ;
    rdfs:comment "Work that has been translated, i.e., the text expressed in a language different from that of the original work."@en ;
    rdfs:range lite:Resource ;
    rdfs:domain lite:Resource .

rel:hasAdaptation a rdf:Property ;
    rdfs:label "has adaptation"@en ;
    rdfs:comment "Target resource is an adaptation of the source resource."@en ;
    rdfs:range lite:Resource ;
    rdfs:domain lite:Resource .

rel:hasTranslation a rdf:Property ;
    rdfs:label "has translation"@en ;
    rdfs:comment "Work that translates the text of the source entity into a language different from that of the original."@en ;
    rdfs:range lite:Resource ;
    rdfs:domain lite:Resource .

rel:mergesWith a rdf:Property ;
    rdfs:label "merges with"@en ;
    rdfs:comment "Two or more resources combine to create a single resource."@en ;
    rdfs:domain lite:Resource ;
    rdfs:range lite:Resource .

rel:mergedWith a rdf:Property ;
    rdfs:label "merged with"@en ;
    rdfs:comment "One of two or more works that come together to form a new work."@en ;
    rdfs:domain lite:Resource ;
    rdfs:range lite:Resource .

rel:separatedFrom a rdf:Property ;
    rdfs:label "separated from"@en ;
    rdfs:comment "Work that spun off a part of its content to form a new work."@en ;
    rdfs:domain lite:Resource ;
    rdfs:range lite:Resource .

rel:splitInto a rdf:Property ;
    rdfs:label "split into"@en ;
    rdfs:comment "One of two or more works resulting from the division of an earlier work into separate works."@en ;
    rdfs:domain lite:Resource ;
    rdfs:range lite:Resource .

rel:supersedes a rdf:Property ;
    rdfs:label "supersedes"@en ;
    rdfs:comment "Earlier work whose content has been replaced by a later work, usually because the later work contains updated or new information."@en ;
    rdfs:domain lite:Resource ;
    rdfs:range lite:Resource .

rel:supersededBy a rdf:Property ;
    rdfs:label "superseded by"@en ;
    rdfs:comment "Later Work used in place of an earlier work, usually because the later work contains updated or new information."@en ;
    rdfs:domain lite:Resource ;
    rdfs:range lite:Resource .

rel:supersedesInPart a rdf:Property ;
    rdfs:label "supersedes in part"@en ;
    rdfs:comment "Earlier work whose content has been partially replaced by a later work, usually because the later work contains updated or new information."@en ;
    rdfs:domain lite:Resource ;
    rdfs:range lite:Resource .

rel:supersededInPartBy a rdf:Property ;
    rdfs:label "superseded in part by"@en ;
    rdfs:comment "Resource has been partially superseded by another resource."@en ;
    rdfs:domain lite:Resource ;
    rdfs:range lite:Resource .

rel:unionOf a rdf:Property ;
    rdfs:label "union of"@en ;
    rdfs:comment "One of two or more works which came together to form a new work."@en ;
    rdfs:domain lite:Resource ;
    rdfs:range lite:Resource .

## Relationships derived from MARC relator terms

rel:abridger a rdf:Property ;
    rdfs:label "abridger"@en ;
    rdfs:comment "Professional contributing to a resource by shortening or condensing the original work but leaving the nature and content of the original work substantially unchanged."@en ;
    rdfs:domain lite:Resource ;
    rdfs:range lite:Resource .

rel:actor a rdf:Property ;
    rdfs:label "actor"@en ;
    rdfs:comment "Performer contributing to an expression of a work by acting as a cast member or player in a musical or dramatic presentation, etc."@en ;
    rdfs:domain lite:Resource ;
    rdfs:range lite:Resource .

rel:adapter a rdf:Property ;
    rdfs:label "adapter"@en ;
    rdfs:comment "Person or organization who 1) reworks a musical composition, usually for a different medium, or 2) rewrites novels or stories for motion pictures or other audiovisual medium."@en ;
    rdfs:domain lite:Resource ;
    rdfs:range lite:Resource .

rel:addressee a rdf:Property ;
    rdfs:label "addressee"@en ;
    rdfs:comment "Person, family, or organization to whom the correspondence in a work is addressed."@en ;
    rdfs:domain lite:Resource ;
    rdfs:range lite:Resource .

rel:analyst a rdf:Property ;
    rdfs:label "analyst"@en ;
    rdfs:comment "Person or organization that reviews, examines and interprets data or information in a specific area."@en ;
    rdfs:domain lite:Resource ;
    rdfs:range lite:Resource .

rel:animator a rdf:Property ;
    rdfs:label "animator"@en ;
    rdfs:comment "Person contributing to a moving image work or computer program by giving apparent movement to inanimate objects or drawings."@en ;
    rdfs:domain lite:Resource ;
    rdfs:range lite:Resource .

rel:annotator a rdf:Property ;
    rdfs:label "annotator"@en ;
    rdfs:comment "Person who makes manuscript annotations on an item."@en ;
    rdfs:domain lite:Resource ;
    rdfs:range lite:Resource .

rel:appellant a rdf:Property ;
    rdfs:label "appellant"@en ;
    rdfs:comment "Person or organization who appeals a lower court's decision."@en ;
    rdfs:domain lite:Resource ;
    rdfs:range lite:Resource .

rel:appellee a rdf:Property ;
    rdfs:label "appellee"@en ;
    rdfs:comment "Person or organization against whom an appeal is taken."@en ;
    rdfs:domain lite:Resource ;
    rdfs:range lite:Resource .

rel:applicant a rdf:Property ;
    rdfs:label "applicant"@en ;
    rdfs:comment "Person or organization responsible for the submission of an application or who is named as eligible for the results of the processing of the application (e.g., bestowing of rights, reward, title, position)."@en ;
    rdfs:domain lite:Resource ;
    rdfs:range lite:Resource .

rel:appraiser a rdf:Property ;
    rdfs:label "appraiser"@en ;
    rdfs:comment "Professional who evaluates and determines the value of property, assets, or goods, often for purposes such as insurance, taxation, or sale."@en ;
    rdfs:domain lite:Resource ;
    rdfs:range lite:Resource .

rel:architect a rdf:Property ;
    rdfs:label "architect"@en ;
    rdfs:comment "Professional responsible for creating an architectural design, including a pictorial representation intended to show how a building, etc., will look when completed. Architects also oversees the construction of structures."@en ;
    rdfs:domain lite:Resource ;
    rdfs:range lite:Resource .

rel:arranger a rdf:Property ;
    rdfs:label "arranger"@en ;
    rdfs:comment "Professional contributing to a musical work by rewriting the composition for a medium of performance different from that for which the work was originally intended, or modifying the work for the same medium of performance, etc., such that the musical substance of the original composition remains essentially unchanged. For extensive modification that effectively results in the creation of a new musical work, see composer."@en ;
    rdfs:domain lite:Resource ;
    rdfs:range lite:Resource .

rel:arrangerOfMusic a rdf:Property ;
    rdfs:label "arranger of music"@en ;
    rdfs:comment "Professional musician who adapts and organizes musical compositions, modifying elements like instrumentation, harmony, or structure to suit a particular performance or style."@en ;
    rdfs:domain lite:Resource ;
    rdfs:range lite:Resource .

rel:graphicTechnician a rdf:Property ;
    rdfs:label "graphic technician"@en ;
    rdfs:comment "Professional who operates and maintains graphic equipment, designs visual content, and ensures the quality of printed or digital media."@en ;
    rdfs:domain lite:Resource ;
    rdfs:range lite:Resource .

    ## Note to self: I stopped at artcopyist on 9/22/24